corrections on the driver

veluslib.ml
@@ -84,4 +84,3 @@ let add_builtin p (name, (out, ins, b)) =
 
 let add_builtins p =
   List.fold_left add_builtin p C2C.builtins_generic.Builtins.functions
-
